proof/invariant-abstract/DetSchedAux_AI.thy
@@ -81,6 +81,31 @@ lemma retype_region_etcb_at:"\<lbrace>(\<lambda>s. etcb_at P t s) and valid_etcb
   apply (clarsimp simp add: pred_tcb_at_def obj_at_def simp del: fun_upd_apply)
   apply (blast intro: retype_etcb_at_helper)
   done
+(*
+lemma retype_bound_sc_tcb_at_helper:
+   "\<lbrakk>valid_etcbs s; kheap s t = Some (TCB tcb);
+        P (tcb_sched_context tcb); d \<noteq> Untyped\<rbrakk>
+       \<Longrightarrow> foldr (\<lambda>p kh. kh(p \<mapsto> default_object d dev c))
+             ptrs
+             (kheap s) t =
+            Some (TCB tcb) \<and>
+            (\<exists>tcba. TCB tcb = TCB tcba \<and> P (tcb_sched_context tcba))"
+  apply (induct ptrs)
+  apply simp
+  apply (case_tac d)
+  apply (clarsimp split: if_split_asm simp: default_tcb_def default_object_def default_ext_def etcb_at'_def)+
+  done
+
+lemma retype_region_bound_sc_tcb_at:
+  "\<lbrace>(\<lambda>s::det_ext state. bound_sc_tcb_at (\<lambda>sc. sc = Some scp) t s) and K (scp \<notin> set (retype_addrs a d b c))\<rbrace>
+     retype_region a b c d dev \<lbrace>\<lambda>r s. (*st_tcb_at (Not o inactive) t s \<longrightarrow>*) bound_sc_tcb_at (\<lambda>sc. sc = Some scp) t s\<rbrace> "
+  apply (simp add: retype_region_def)
+  apply (simp add: retype_region_ext_def bind_assoc)
+  apply wp
+  apply (clarsimp simp add: pred_tcb_at_def obj_at_def simp del: fun_upd_apply)
+  apply (rule_tac x="TCB tcb" in exI)
+  apply (blast intro: retype_etcb_at_helper)
+  done*)
 
 lemma retype_region_valid_etcbs[wp]:"\<lbrace>valid_etcbs\<rbrace> retype_region a b c d dev \<lbrace>\<lambda>_. valid_etcbs\<rbrace>"
   apply (simp add: retype_region_def)
@@ -135,6 +160,12 @@ locale DetSchedAux_AI =
     "\<And>P i. \<lbrace>\<lambda>s::'state_ext state. P (cur_thread s)\<rbrace> invoke_untyped i \<lbrace>\<lambda>_ s. P (cur_thread s)\<rbrace>"
   assumes invoke_untyped_idle_thread[wp]:
     "\<And>P i. \<lbrace>\<lambda>s::'state_ext state. P (idle_thread s)\<rbrace> invoke_untyped i \<lbrace>\<lambda>_ s. P (idle_thread s)\<rbrace>"
+  assumes invoke_untyped_bound_sc[wp]:
+    "\<And>P i t. \<lbrace>\<lambda>s::'state_ext state. (invs and st_tcb_at ((Not \<circ> inactive) and (Not \<circ> idle)) t
+       and bound_sc_tcb_at P t and ct_active and valid_untyped_inv i) s\<rbrace> invoke_untyped i \<lbrace>\<lambda>_ s. bound_sc_tcb_at P t s\<rbrace>"
+  assumes invoke_untyped_schedulable_tcb_at[wp]:
+    "\<And>i t. \<lbrace>\<lambda>s::'state_ext state. (invs and st_tcb_at ((Not \<circ> inactive) and (Not \<circ> idle)) t
+       and schedulable_tcb_at t and ct_active and valid_untyped_inv i) s\<rbrace> invoke_untyped i \<lbrace>\<lambda>_ s. schedulable_tcb_at t s\<rbrace>"
 
 locale DetSchedAux_AI_det_ext = DetSchedAux_AI "TYPE(det_ext)" +
   assumes delete_objects_etcb_at[wp]:
@@ -217,6 +248,7 @@ end
 lemma valid_sched_tcb_state_preservation:
   assumes st_tcb: "\<And>P t. \<lbrace>I and ct_active and st_tcb_at (P and Not o inactive and Not o idle) t\<rbrace> f \<lbrace>\<lambda>_.st_tcb_at P t\<rbrace>"
   assumes stuff: "\<And>P t. \<lbrace>(\<lambda>s. etcb_at P t s) and valid_etcbs\<rbrace> f \<lbrace>\<lambda>r s. st_tcb_at (Not o inactive) t s \<longrightarrow> etcb_at P t s\<rbrace>"
+  assumes bound_sc: "\<And>t. \<lbrace>\<lambda>s. schedulable_tcb_at t s\<rbrace> f \<lbrace>\<lambda>rv s. schedulable_tcb_at t s\<rbrace>"
   assumes cur_thread: "\<And>P. \<lbrace>\<lambda>s. P (cur_thread s)\<rbrace> f \<lbrace>\<lambda>r s. P (cur_thread s)\<rbrace>"
   assumes idle_thread: "\<And>P. \<lbrace>\<lambda>s. P (idle_thread s)\<rbrace> f \<lbrace>\<lambda>r s. P (idle_thread s)\<rbrace>"
   assumes valid_etcb: "\<lbrace>valid_etcbs\<rbrace> f \<lbrace>\<lambda>_. valid_etcbs\<rbrace>"
@@ -269,11 +301,113 @@ lemma valid_sched_tcb_state_preservation:
    apply (case_tac "itcb_state tcb"; simp)
   apply (rule conjI)
    apply clarsimp
+  apply (rule conjI)
    apply (rule_tac use_valid[OF _ st_tcb],assumption)
    apply simp
   apply (erule pred_tcb_weakenE)
    apply simp
    apply (case_tac "itcb_state tcb", simp+)
+   apply (rule_tac use_valid[OF _ bound_sc],assumption)
+   apply simp
+  apply (rule conjI)
+   apply (clarsimp simp: switch_in_cur_domain_def in_cur_domain_def)
+   apply (rule use_valid[OF _ stuff, rule_format], assumption)
+    apply simp
+   apply (rule use_valid[OF _ st_tcb], assumption)
+   apply simp
+   apply (erule st_tcb_weakenE)
+   apply (case_tac st, simp+)
+  apply (clarsimp simp: ct_in_cur_domain_2_def in_cur_domain_2_def)
+  apply (frule_tac P1="\<lambda>idle. idle = (idle_thread s)" in use_valid[OF _ idle_thread], simp)
+  apply (rule conjI)
+   apply (rule impI)
+   apply (simp, erule disjE, simp)
+   apply (frule_tac P1="(\<lambda>t. tcb_domain t = cur_domain s)" and t1="cur_thread s" in use_valid[OF _ stuff])
+    apply (clarsimp simp: etcb_at_def split: option.splits)
+   apply clarsimp
+   apply (erule notE, rule use_valid[OF _ st_tcb],assumption)
+   apply (simp add: ct_in_state_def)
+   apply (erule st_tcb_weakenE)
+   apply simp
+   apply (case_tac st, simp+)
+  apply(frule (1) use_valid[OF _ valid_idle])
+  apply(simp add: valid_idle_etcb_def)
+  apply(frule use_valid[OF _ stuff[where t=idle_thread_ptr]])
+   apply simp
+  apply(erule mp)
+  apply(fastforce simp: valid_idle_def pred_tcb_at_def obj_at_def)
+  done
+
+(*Leverages the fact that retype only clears out inactive tcbs under
+  the invariants*)
+lemma valid_sched_tcb_state_preservation_gen:
+  assumes st_tcb: "\<And>P t. \<lbrace>I and ct_active and st_tcb_at (P and Not o inactive and Not o idle) t\<rbrace> f \<lbrace>\<lambda>_.st_tcb_at P t\<rbrace>"
+  assumes stuff: "\<And>P t. \<lbrace>(\<lambda>s. etcb_at P t s) and valid_etcbs\<rbrace> f \<lbrace>\<lambda>r s. st_tcb_at (Not o inactive) t s \<longrightarrow> etcb_at P t s\<rbrace>"
+  assumes bound_sc:
+            "\<And>Q t. \<lbrace>I and ct_active and st_tcb_at (Not o inactive and Not o idle) t and schedulable_tcb_at t\<rbrace>
+                                 f \<lbrace>\<lambda>_.schedulable_tcb_at t\<rbrace>"
+(*  assumes bound_sc: "\<And>Q t. \<lbrace>\<lambda>s. bound_sc_tcb_at Q t s\<rbrace> f \<lbrace>\<lambda>rv s. bound_sc_tcb_at Q t s\<rbrace>"*)
+  assumes cur_thread: "\<And>P. \<lbrace>\<lambda>s. P (cur_thread s)\<rbrace> f \<lbrace>\<lambda>r s. P (cur_thread s)\<rbrace>"
+  assumes idle_thread: "\<And>P. \<lbrace>\<lambda>s. P (idle_thread s)\<rbrace> f \<lbrace>\<lambda>r s. P (idle_thread s)\<rbrace>"
+  assumes valid_etcb: "\<lbrace>valid_etcbs\<rbrace> f \<lbrace>\<lambda>_. valid_etcbs\<rbrace>"
+  assumes valid_blocked: "\<lbrace>valid_blocked\<rbrace> f \<lbrace>\<lambda>_. valid_blocked\<rbrace>"
+  assumes valid_idle: "\<lbrace>I\<rbrace> f \<lbrace>\<lambda>_. valid_idle\<rbrace>"
+  assumes valid_others: "\<And>P. \<lbrace>\<lambda>s. P (scheduler_action s) (ready_queues s) (cur_domain s)\<rbrace> f \<lbrace>\<lambda>r s. P (scheduler_action s) (ready_queues s) (cur_domain s)\<rbrace>"
+  shows "\<lbrace>I and ct_active and valid_sched and valid_idle\<rbrace> f \<lbrace>\<lambda>_. valid_sched\<rbrace>"
+  apply (clarsimp simp add: valid_sched_def valid_def)
+  apply (frule(1) use_valid[OF _ valid_etcb])
+  apply (frule(1) use_valid[OF _ valid_blocked])
+  apply simp
+  apply (frule_tac P1="\<lambda>sa rq cdom. rq = ready_queues s \<and> sa = scheduler_action s \<and> cdom = cur_domain s" in use_valid[OF _ valid_others])
+   apply simp
+  apply (rule conjI)
+   apply (clarsimp simp add: valid_queues_def)
+   apply (drule_tac x=d in spec)
+   apply (drule_tac x=p in spec)
+   apply clarsimp
+   apply (drule_tac x=t in bspec)
+    apply simp
+   apply clarsimp
+   apply (subgoal_tac "st_tcb_at runnable t b")
+    apply simp
+    apply (rule conjI)
+     apply (fastforce simp: valid_etcbs_def pred_tcb_at_def obj_at_def)
+    apply (frule_tac P1="(\<lambda>t. tcb_priority t = p \<and> tcb_domain t = d)" and t1=t in use_valid[OF _ stuff])
+     apply simp
+    apply (simp add: pred_tcb_at_def obj_at_def)
+    apply force
+   apply (rule_tac use_valid[OF _ st_tcb],assumption)
+   apply simp
+   apply (erule pred_tcb_weakenE)
+   apply simp
+   apply (case_tac "itcb_state tcb")
+          apply simp+
+  apply (frule_tac P1="\<lambda>ct. ct = (cur_thread s)" in use_valid[OF _ cur_thread])
+   apply simp
+  apply (rule conjI)
+   apply simp
+  apply simp
+  apply (clarsimp simp add: valid_sched_action_def is_activatable_def weak_valid_sched_action_def)
+  apply (rule conjI)
+   apply clarsimp
+   apply (frule_tac P1="active" and t1="cur_thread s" in use_valid[OF _ st_tcb])
+    apply (simp add: ct_in_state_def)
+    apply (erule pred_tcb_weakenE)
+    apply simp
+    apply (case_tac "itcb_state tcb"; simp)
+   apply (erule pred_tcb_weakenE)
+   apply (case_tac "itcb_state tcb"; simp)
+  apply (rule conjI)
+   apply clarsimp
+  apply (rule conjI)
+   apply (rule_tac use_valid[OF _ st_tcb],assumption)
+   apply simp
+  apply (erule pred_tcb_weakenE)
+   apply simp
+   apply (case_tac "itcb_state tcb", simp+)
+   apply (rule_tac use_valid[OF _ bound_sc],assumption)
+   apply simp
+  apply (erule pred_tcb_weakenE, fastforce)
   apply (rule conjI)
    apply (clarsimp simp: switch_in_cur_domain_def in_cur_domain_def)
    apply (rule use_valid[OF _ stuff, rule_format], assumption)
@@ -319,10 +453,10 @@ lemma invoke_untyped_valid_sched:
   including no_pre
   apply (rule hoare_pre)
    apply (rule_tac I="invs and valid_untyped_inv ui and ct_active"
-     in valid_sched_tcb_state_preservation)
+     in valid_sched_tcb_state_preservation_gen)
           apply (wp invoke_untyped_st_tcb_at)
           apply simp
-         apply (wp invoke_untyped_etcb_at)+
+         apply (wpsimp wp: invoke_untyped_etcb_at)+
     apply (rule hoare_post_impErr, rule hoare_pre, rule invoke_untyp_invs,
         simp_all add: invs_valid_idle)[1]
    apply (rule_tac f="\<lambda>s. P (scheduler_action s)" in hoare_lift_Pf)
@@ -337,6 +471,33 @@ lemmas hoare_imp_lift_something = hoare_convert_imp
 
 crunch valid_queues[wp]: create_cap,cap_insert valid_queues
   (wp: valid_queues_lift)
+
+lemma schedulable_tcb_at_cde_update[simp]:
+  "schedulable_tcb_at t (s\<lparr>cdt := param_a\<rparr>) = schedulable_tcb_at t s"
+  by (clarsimp simp: schedulable_tcb_at_def)
+
+lemma schedulable_tcb_at_cde_list_update[simp]:
+  "schedulable_tcb_at t (s\<lparr>cdt_list := param_a\<rparr>) = schedulable_tcb_at t s"
+  by (clarsimp simp: schedulable_tcb_at_def)
+
+lemma schedulable_tcb_at_is_original_cap_update[simp]:
+  "schedulable_tcb_at t (s\<lparr>is_original_cap := param_a\<rparr>) = schedulable_tcb_at t s"
+  by (clarsimp simp: schedulable_tcb_at_def)
+
+
+lemma set_cap_schedulable_tcb_at[wp]:
+ "\<lbrace>schedulable_tcb_at t\<rbrace> set_cap c p \<lbrace>\<lambda>rv. schedulable_tcb_at t\<rbrace>"
+  apply (simp add: set_cap_def set_object_def split_def)
+  apply (wp get_object_wp | wpc)+
+  apply (clarsimp simp: schedulable_tcb_at_def pred_tcb_at_def obj_at_def
+       | intro impI conjI | rule_tac x=scp in exI)+
+  done
+
+crunch schedulable_tcb_at[wp]: create_cap,cap_insert_ext "schedulable_tcb_at t :: det_ext state \<Rightarrow> bool"
+  (simp: crunch_simps)
+
+crunch schedulable_tcb_at[wp]: cap_insert "schedulable_tcb_at t :: det_ext state \<Rightarrow> bool"
+  (simp: crunch_simps wp: hoare_drop_imps)
 
 crunch valid_sched_action[wp]: create_cap,cap_insert valid_sched_action
   (wp: valid_sched_action_lift)
